proof/Progress.v
@@ -1,6 +1,82 @@
 
 Require Import TyJudge.
 Require Import EvJudge.
+Require Import FunctionalExtensionality.
+
+Theorem closed_var_not
+ : forall n
+ , ~(closed (XVar n)).
+Proof.
+ intro. unfold not. intro.
+ unfold closed in H.
+ specialize H with n. contradict H. apply FreeX_var.
+Qed.
+
+
+Theorem functional_extensionality_not
+ : forall A B (f : A -> B) (g : A -> B)
+ , (exists x, f x <> g x) -> f <> g.
+Proof.
+ intros. unfold not. intro. subst.
+ inversion H. contradiction H0.
+ trivial.
+Qed.
+
+
+Theorem check_closed_in_empty
+ : forall env t T 
+ , closed t -> TYPE env t T -> TYPE empty t T.
+Proof.
+ intros.
+ eapply tyenv_invariance.
+ apply H0.
+ intros. contradict H1. unfold closed in H. apply H.
+Qed.
+
+
+Theorem closed_lam
+ : forall x T t 
+ , closed t -> closed (XLam x T t).
+Proof. 
+ intros. unfold closed. intros. unfold not. intro.
+ inversion H0. subst.
+ unfold closed in H. apply H in H6. assumption.
+Qed.
+
+
+Theorem closed_app
+ : forall t1 t2
+ , closed t1 -> closed t2 -> closed (XApp t1 t2).
+Proof. 
+ intros.
+ unfold closed. intros. unfold not. intro.
+ unfold closed in H.  specialize H  with x.
+ unfold closed in H0. specialize H0 with x.
+ inversion H1. subst. auto. subst. auto.
+Qed.
+
+
+Theorem check_empty_is_closed
+ : forall t T
+ , TYPE empty t T -> closed t.
+Proof.
+ intros t T.
+ generalize T.
+ induction t.
+ Case "XVar".
+  intros. inversion H. subst. unfold empty in H2. inversion H2.
+ Case "XLam".
+  intros. inversion H. subst.
+  unfold closed. intro.
+  unfold not. intro.
+  eapply tyenv_contains_free_vars with (x:=x) in H.
+  inversion H. inversion H1. assumption.
+ Case "XApp".
+  intros. inversion H. subst.
+  apply closed_app.
+  eapply IHt1. apply H3.
+  eapply IHt2. apply H5.
+Qed.
 
 
 Theorem progress
@@ -12,24 +88,26 @@ Proof.
  remember (@empty ty) as G.
  induction Ht.
  Case "XVar".
-  left. subst. inversion H.
+  left. subst. inversion H. subst.
  Case "XLam".
-  left. auto.
+  left. apply VALUE_XLam.
+  apply TYLam in Ht.
+  eapply check_empty_is_closed. apply Ht.
  Case "XApp".
   right.
-  destruct IHHt1. auto. 
+  destruct IHHt1. assumption. 
   SCase "t1 value".
-   destruct H. destruct IHHt2. trivial.
+   destruct H. destruct IHHt2. assumption.
    SSCase "t2 value".
-    exists (subst x t2 t). apply EVAppAbs. trivial.
+    exists (subst x t2 t). apply EVAppAbs. assumption.
    SSCase "t2 steps".
-    destruct H as [t2' Htsp].
+    destruct H0 as [t2' Htsp].
     exists (XApp (XLam x T t) t2').
-    apply EVApp2. trivial. trivial.
+    apply EVApp2. apply VALUE_XLam. assumption. assumption.
   SCase "t1 steps".
    destruct H as [t1' Htsp].
    exists (XApp t1' t2).
-   apply EVApp1. trivial.
+   apply EVApp1. assumption.
 Qed.
 
 
